publish changes from instructor-

chapter05-dsm/exercises/exercise03.dfy
@@ -3,38 +3,14 @@
 
 // TODO(manos): how should we ensure this file is disseminated at the
 // appropriate time, so students aren't waiting for it?
-//
-// Please begin with a copy of the official solution to exercises 01 & 02,
-// to ensure you're not doing battle with mistakes in your own protocol definition.
-// The proof is challenging enough for an exercise without fighting protocol bugs.
-include "exercise02-solution.dfy"
+
+include "model_for_ex03.dfy"
 
 module Proof {
   import opened Types
   import opened Library
   import opened DistributedSystem
   import opened Obligations
-
-  predicate VoteMessagesAgreeWithParticipantPreferences(c: Constants, v: Variables)
-    requires Host.GroupWF(c.hosts, v.hosts)
-  {
-    (forall msg |
-      && msg in v.network.sentMsgs
-      && msg.VoteMsg?
-      && ValidParticipantId(c, msg.sender)
-      :: msg.vote == ParticipantConstants(c, msg.sender).preference
-    )
-  }
-
-  predicate CoordinatorStateSupportedByVote(c: Constants, v: Variables)
-    requires Host.GroupWF(c.hosts, v.hosts)
-  {
-    (forall idx:HostId |
-      && ValidParticipantId(c, idx)
-      && CoordinatorVars(c, v).votes[idx].Some?
-      :: VoteMsg(idx, CoordinatorVars(c, v).votes[idx].value) in v.network.sentMsgs
-    )
-  }
 
   predicate DecisionMsgsAgreeWithDecision(c: Constants, v: Variables)
     requires Host.GroupWF(c.hosts, v.hosts)
@@ -49,9 +25,9 @@ module Proof {
   predicate Inv(c: Constants, v: Variables)
   {
     && Host.GroupWF(c.hosts, v.hosts)
-    && VoteMessagesAgreeWithParticipantPreferences(c, v)
-    && CoordinatorStateSupportedByVote(c, v)
+    // We'll give you one invariant to get you started...
     && DecisionMsgsAgreeWithDecision(c, v)
+    // ...but you'll need more.
     && Safety(c, v)
   }
 
@@ -59,9 +35,6 @@ module Proof {
     requires Init(c, v)
     ensures Inv(c, v)
   {
-    // Nobody has agreed with anything yet, so they agree with both.
-    assert AllWithDecisionAgreeWithThisOne(c, v, Commit); // witness.
-    assert AllWithDecisionAgreeWithThisOne(c, v, Abort); // witness.
   }
 
   lemma InvInductive(c: Constants, v: Variables, v': Variables)
@@ -69,25 +42,6 @@ module Proof {
     requires Next(c, v, v')
     ensures Inv(c, v')
   {
-    // The body of this lemma got really big (expanding foralls, case splits,
-    // testing asserts) while I was figuring out what invariants were missing
-    // ... and fixing a couple of errors in the protocol definition itself.
-    // Afterward, nearly all of that text could be deleted.
-
-    var step :| NextStep(c, v, v', step);   // Witness
-
-    // sklomize msg from DecisionMsgsAgreeWithDecision
-    forall msg |
-      && msg in v'.network.sentMsgs
-      && msg.DecisionMsg?
-      ensures CoordinatorHost.ObservesResult(CoordinatorConstants(c), CoordinatorVars(c, v'), msg.decision)
-    {
-      var hostid := step.hostid;
-      assert Host.Next(c.hosts[hostid], v.hosts[hostid], v'.hosts[hostid], step.msgOps);  // observe trigger
-      if msg in v.network.sentMsgs {  // observe trigger
-      }
-    }
-    assert Safety(c, v'); // somehow this trigger is necessary to get the forall above! Bizarre.
   }
 
   lemma InvImpliesSafety(c: Constants, v: Variables)
