chapter05-dsm/exercises/model_for_ex03.dfy
@@ -1,0 +1,516 @@
+// This file is an "official solution" to exercises 01 & 02, to ensure you're
+// not doing battle with mistakes in your own protocol definition.  The proof
+// is challenging enough for an exercise without fighting protocol bugs.
+
+/*
+ * 2PC should satisfy the Atomic Commit specification. English design doc:
+ *
+ * AC-1: All processes that reach a decision reach the same one.
+ * AC-3: The Commit decision can only be reached if all processes prefer Yes.
+ * AC-4: If all processes prefer Yes, then the decision must be Commit.
+ *
+ * Note that the full Atomic Commit spec includes these additional properties,
+ * but you should ignore them for this exercise:
+ * AC-2: (stability) A process cannot reverse its decision after it has reached one.
+ *       (best modeled with refinement)
+ * AC-5: (liveness) All processes eventually decide.
+ *
+ */
+
+// Note that we include the result of exercise01. If you have doubts about the
+// model you built there, please contact an instructor for a correct solution
+// to build on for this exercise.
+
+/*
+ * 2-Phase Commit Protocol english design doc:
+ *
+ * 1, Coordinator sends VOTE-REQ to all participants.
+ * 2. Each participant i sends back vote_i to coordinator.
+ *   If vote_i=No then i sets decision_i := Abort.
+ * 3. Coordinator collects votes.
+ *   If all votes are yes then coordinator sets decision_c := Commit and sends
+ *   Commit to all participants.
+ *   Else coordinator sets decision_c := Abort and sends Abort to all
+ *   participants who voted yes.
+ * 4. Participants receiving Commit set decision_i := Commit
+ *   (The slide is delightfully poorly specified. "else decision_i := Abort"!?
+ *   When else? As soon as it doesn't hear Commit!?)
+ *
+ * This file provides a lot of helpful framework. You only need to
+ * define Types.Message and then fill in the state machine types and actions
+ * in module CoordinatorHost and module ParticipantHost.
+ */
+
+include "../../library/Library.dfy" // Some handy utilities.
+
+module Types {
+  import opened Library
+
+  type HostId = nat
+  datatype Vote = Yes | No
+  datatype Decision = Commit | Abort
+
+  // Have to define our message datatype so network can refer to it.
+  // (There are cleverer ways to parameterize the network module, but
+  // we're trying to avoid getting fancy with the Dafny module system.)
+  datatype Message =
+    | VoteReqMsg                           // from leader
+    | VoteMsg(sender: HostId, vote: Vote)  // from participant
+    | DecisionMsg(decision: Decision)
+
+  // A MessageOps is a "binding variable" used to connect a Host's Next step
+  // (what message got received, what got sent?) with the Network (only allow
+  // receipt of messages sent prior; record newly-sent messages).
+  // Note that both fields are Option. A step predicate can say recv.None?
+  // to indicate that it doesn't need to receive a message to occur.
+  // It can say send.None? to indicate that it doesn't want to transmit a message.
+  datatype MessageOps = MessageOps(recv:Option<Message>, send:Option<Message>)
+}
+
+// There are two host roles in 2PC, Coordinator and Participant. We'll define
+// separate state machines for each.
+// This state machine defines how a coordinator host should behave: what state
+// it records, and what actions it's allowed to take in response to incoming
+// messages (or spontaneously by thinking about its existing state).
+module CoordinatorHost {
+  import opened Types
+  import opened Library
+
+  datatype Constants = Constants(participantCount: nat)
+
+  // What relationship must hold between this host's own constants and the
+  // structure of the overall group of hosts? It needs to have a correct
+  // count of the number of participants.
+  predicate ConstantsValidForGroup(c: Constants, participantCount: nat)
+  {
+    && c.participantCount == participantCount
+  }
+
+  datatype Variables = Variables(votes: seq<Option<Vote>>, decision: Option<Decision>)
+  {
+    // WF is for a simple condition that relates every valid Variables state
+    // to the Constants.
+    predicate WF(c: Constants) {
+      && |votes| == c.participantCount
+    }
+  }
+
+  predicate Init(c: Constants, v: Variables)
+  {
+    && v.WF(c)
+    // No votes recorded yet
+    && (forall hostIdx:HostId | hostIdx < |v.votes| :: v.votes[hostIdx].None?)
+    // No decision recorded yet
+    && v.decision.None?
+  }
+
+  // Protocol steps. Define an action predicate for each step of the protocol
+  // that the coordinator is involved in.
+  // Hint: it's probably easiest to separate the receipt and recording of
+  // incoming votes from detecting that all have arrived and making a decision.
+  predicate SendReq(c: Constants, v: Variables, v': Variables, msgOps: MessageOps)
+  {
+    && v.WF(c)
+    && v'.WF(c)
+    && msgOps == MessageOps(None, Some(VoteReqMsg))
+    && v' == v  // UNCHANGED everything.
+  }
+
+  predicate LearnVote(c: Constants, v: Variables, v': Variables, msgOps: MessageOps)
+  {
+    && v.WF(c)
+    && v'.WF(c)
+    && msgOps.recv.Some?
+    && var recvMsg := msgOps.recv.value;
+    && recvMsg.VoteMsg?
+    && recvMsg.sender < c.participantCount
+    // Record sender's vote.
+    && v' == v.(votes := v.votes[recvMsg.sender := Some(recvMsg.vote)])
+    && msgOps.send.None?
+  }
+
+  predicate AllVotesCollected(c: Constants, v: Variables)
+  {
+    && v.WF(c)
+    && (forall hostIdx:HostId | hostIdx < |v.votes| :: v.votes[hostIdx].Some?)
+  }
+
+  predicate ObservesResult(c: Constants, v: Variables, decision: Decision)
+  {
+    && v.WF(c)
+    && AllVotesCollected(c, v)
+    && decision ==
+      if (forall hostIdx:HostId | hostIdx < |v.votes| :: v.votes[hostIdx].value.Yes?)
+      then Commit
+      else Abort
+  }
+
+  predicate Decide(c: Constants, v: Variables, v': Variables, decision: Decision, msgOps: MessageOps)
+  {
+    && v.WF(c)
+    && v'.WF(c)
+    && msgOps.recv.None?
+    && ObservesResult(c, v, decision)
+    // Record the decision
+    && v' == v.(decision := Some(decision))
+    // Transmit the decision
+    && msgOps.send == Some(DecisionMsg(decision))
+  }
+
+  // JayNF
+  datatype Step =
+    | SendReqStep
+    | LearnVoteStep
+    | DecideStep(decision: Decision)
+
+  // msgOps is a "binding variable" -- the host and the network have to agree
+  // on its assignment to make a valid transition. So the host explains what
+  // would happen if it could receive a particular message, and the network
+  // decides whether such a message is available for receipt.
+  predicate NextStep(c: Constants, v: Variables, v': Variables, step: Step, msgOps: MessageOps)
+  {
+    match step
+      case SendReqStep => SendReq(c, v, v', msgOps)
+      case LearnVoteStep => LearnVote(c, v, v', msgOps)
+      case DecideStep(decision) => Decide(c, v, v', decision, msgOps)
+  }
+
+  predicate Next(c: Constants, v: Variables, v': Variables, msgOps: MessageOps)
+  {
+    exists step :: NextStep(c, v, v', step, msgOps)
+  }
+}
+
+module ParticipantHost {
+  import opened Types
+  import opened Library
+
+  datatype Constants = Constants(hostId: HostId, preference: Vote)
+
+  // What relationship must hold between this host's own constants and the
+  // structure of the overall group of hosts? It needs to know its hostId.
+  predicate ConstantsValidForGroup(c: Constants, hostId: HostId)
+  {
+    && c.hostId == hostId
+  }
+
+  datatype Variables = Variables(decision: Option<Decision>)
+  {
+    predicate WF(c: Constants) {
+      true
+    }
+  }
+
+  predicate Init(c: Constants, v: Variables)
+  {
+    && v.decision.None?
+  }
+
+  // Protocol steps. Define an action predicate for each step of the protocol
+  // that participant can take.
+  predicate Vote(c: Constants, v: Variables, v': Variables, msgOps: MessageOps)
+  {
+    && msgOps.recv.Some?
+    && var recvMsg := msgOps.recv.value;
+    && recvMsg.VoteReqMsg?
+    && msgOps.send == Some(VoteMsg(c.hostId, c.preference))
+    // Infer Abort decision if we're voting No
+    && v'.decision == if c.preference.No? then Some(Abort) else v.decision
+  }
+
+  predicate LearnDecision(c: Constants, v: Variables, v': Variables, msgOps: MessageOps)
+  {
+    && msgOps.recv.Some?
+    && var recvMsg := msgOps.recv.value;
+    && recvMsg.DecisionMsg?
+    && v'.decision == Some(recvMsg.decision)
+    && msgOps.send.None?
+  }
+
+  // JayNF
+  datatype Step =
+    | VoteStep
+    | LearnDecisionStep
+
+  predicate NextStep(c: Constants, v: Variables, v': Variables, step: Step, msgOps: MessageOps)
+  {
+    match step
+      case VoteStep => Vote(c, v, v', msgOps)
+      case LearnDecisionStep => LearnDecision(c, v, v', msgOps)
+  }
+
+  predicate Next(c: Constants, v: Variables, v': Variables, msgOps: MessageOps)
+  {
+    exists step :: NextStep(c, v, v', step, msgOps)
+  }
+}
+
+// We define a generic Host as able to be either of the specific roles.
+// This is the ultimate (untrusted) definition of the protocol we're
+// trying to verify.
+// This definition is given to you to clarify how the two protocol roles above
+// are pulled together into the ultimate distributed system.
+module Host {
+  import opened Library
+  import opened Types
+  import CoordinatorHost
+  import ParticipantHost
+
+  datatype Constants =
+    | CoordinatorConstants(coordinator: CoordinatorHost.Constants)
+    | ParticipantConstants(participant: ParticipantHost.Constants)
+
+  datatype Variables =
+    | CoordinatorVariables(coordinator: CoordinatorHost.Variables)
+    | ParticipantVariables(participant: ParticipantHost.Variables)
+  {
+    predicate WF(c: Constants) {
+      && (CoordinatorVariables? <==> c.CoordinatorConstants?) // types of c & v agree
+      // subtype WF satisfied
+      && (match c
+            case CoordinatorConstants(_) => coordinator.WF(c.coordinator)
+            case ParticipantConstants(_) => participant.WF(c.participant)
+          )
+    }
+  }
+
+  // What property must be true of any group of hosts to run the protocol?
+  // Generic DistributedSystem module calls back into this predicate to ensure
+  // that it has a well-formed *group* of hosts.
+  predicate GroupWFConstants(grp_c: seq<Constants>)
+  {
+    // There must at least be a coordinator
+    && 0 < |grp_c|
+    // Last host is a coordinator
+    && Last(grp_c).CoordinatorConstants?
+    // All the others are participants
+    && (forall hostid:HostId | hostid < |grp_c|-1 :: grp_c[hostid].ParticipantConstants?)
+    // The coordinator's constants must correctly account for the number of participants
+    && CoordinatorHost.ConstantsValidForGroup(Last(grp_c).coordinator, |grp_c|-1)
+    // The participants's constants must match their group positions.
+    // (Actually, they just need to be distinct from one another so we get
+    // non-conflicting votes, but this is an easy way to express that property.)
+    && (forall hostid:HostId | hostid < |grp_c|-1
+        :: ParticipantHost.ConstantsValidForGroup(grp_c[hostid].participant, hostid))
+  }
+
+  predicate GroupWF(grp_c: seq<Constants>, grp_v: seq<Variables>)
+  {
+    && GroupWFConstants(grp_c)
+    // Variables size matches group size defined by grp_c
+    && |grp_v| == |grp_c|
+    // Each host is well-formed
+    && (forall hostid:HostId | hostid < |grp_c| :: grp_v[hostid].WF(grp_c[hostid]))
+  }
+
+  // Generic DistributedSystem module calls back into this predicate to give
+  // the protocol an opportunity to set up constraints across the various
+  // hosts.  Protocol requires one coordinator and the rest participants;
+  // coordinator must know how many participants, and participants must know
+  // own ids.
+  predicate GroupInit(grp_c: seq<Constants>, grp_v: seq<Variables>)
+  {
+    // constants & variables are well-formed (same number of host slots as constants expect)
+    && GroupWF(grp_c, grp_v)
+    // Coordinator is inittid to know about the N-1 participants.
+    && CoordinatorHost.Init(Last(grp_c).coordinator, Last(grp_v).coordinator)
+    // Participants initted with their ids.
+    && (forall hostid:HostId | hostid < |grp_c|-1 ::
+        ParticipantHost.Init(grp_c[hostid].participant, grp_v[hostid].participant)
+      )
+  }
+
+  // Dispatch Next to appropriate underlying implementation.
+  predicate Next(c: Constants, v: Variables, v': Variables, msgOps: MessageOps)
+  {
+    && v.WF(c)
+    && v'.WF(c)
+    && (match c
+      case CoordinatorConstants(_) => CoordinatorHost.Next(c.coordinator, v.coordinator, v'.coordinator, msgOps)
+      case ParticipantConstants(_) => ParticipantHost.Next(c.participant, v.participant, v'.participant, msgOps)
+      )
+  }
+}
+
+// The (trusted) model of the environment: There is a network that can only deliver
+// messages that some Host (running the protocol) has sent, but once sent, messages
+// can be delivered repeatedly and in any order.
+// This definition is given to you because it's a common assumption you can
+// reuse. Someday you might decide to assume a different network model (e.g.
+// reliable or at-most-once delivery), but this is a good place to start.
+module Network {
+  import opened Types
+
+  datatype Constants = Constants  // no constants for network
+
+  // Network state is the set of messages ever sent. Once sent, we'll
+  // allow it to be delivered over and over.
+  // (We don't have packet headers, so duplication, besides being realistic,
+  // also doubles as how multiple parties can hear the message.)
+  datatype Variables = Variables(sentMsgs:set<Message>)
+
+  predicate Init(c: Constants, v: Variables)
+  {
+    && v.sentMsgs == {}
+  }
+
+  predicate Next(c: Constants, v: Variables, v': Variables, msgOps: MessageOps)
+  {
+    // Only allow receipt of a message if we've seen it has been sent.
+    && (msgOps.recv.Some? ==> msgOps.recv.value in v.sentMsgs)
+    // Record the sent message, if there was one.
+    && v'.sentMsgs ==
+      v.sentMsgs + if msgOps.send.None? then {} else { msgOps.send.value }
+  }
+}
+
+// The (trusted) model of the distributed system: hosts don't share memory. Each
+// takes its steps independently, interleaved in nondeterministic order with others.
+// They only communicate through the network, and obey the communication model
+// established by the Network model.
+// This is given to you; it can be reused for just about any shared-nothing-concurrency
+// protocol model.
+module DistributedSystem {
+  import opened Library
+  import opened Types
+  import Network
+  import Host
+  import CoordinatorHost
+  import ParticipantHost
+
+  datatype Constants = Constants(
+    hosts: seq<Host.Constants>,
+    network: Network.Constants)
+  {
+    predicate ValidHostId(id: HostId) {
+      id < |hosts|
+    }
+  }
+
+  datatype Variables = Variables(
+    hosts: seq<Host.Variables>,
+    network: Network.Variables)
+
+  predicate Init(c: Constants, v: Variables)
+  {
+    && Host.GroupWF(c.hosts, v.hosts)
+    && Host.GroupInit(c.hosts, v.hosts)
+    && Network.Init(c.network, v.network)
+  }
+
+  predicate HostAction(c: Constants, v: Variables, v': Variables, hostid: HostId, msgOps: MessageOps)
+  {
+    && Host.GroupWF(c.hosts, v.hosts)
+    && Host.GroupWF(c.hosts, v'.hosts)
+    && c.ValidHostId(hostid)
+    && Host.Next(c.hosts[hostid], v.hosts[hostid], v'.hosts[hostid], msgOps)
+    // all other hosts UNCHANGED
+    && (forall otherHost:nat | c.ValidHostId(otherHost) && otherHost != hostid :: v'.hosts[otherHost] == v.hosts[otherHost])
+  }
+
+  // JayNF is pretty simple as there's only a single action disjunct
+  datatype Step =
+    | HostActionStep(hostid: HostId, msgOps: MessageOps)
+
+  predicate NextStep(c: Constants, v: Variables, v': Variables, step: Step)
+  {
+    && HostAction(c, v, v', step.hostid, step.msgOps)
+    // network agrees recv has been sent and records sent
+    && Network.Next(c.network, v.network, v'.network, step.msgOps)
+  }
+
+  predicate Next(c: Constants, v: Variables, v': Variables)
+  {
+    exists step :: NextStep(c, v, v', step)
+  }
+}
+
+module Obligations {
+  import opened Types
+  import opened Library
+  import opened DistributedSystem
+
+  // Here are some handy accessor functions for dereferencing the coordinator
+  // and the participants out of the sequence in Hosts.
+  function CoordinatorConstants(c: Constants) : CoordinatorHost.Constants
+    requires Host.GroupWFConstants(c.hosts)
+  {
+    Last(c.hosts).coordinator
+  }
+
+  function CoordinatorVars(c: Constants, v: Variables) : CoordinatorHost.Variables
+    requires Host.GroupWF(c.hosts, v.hosts)
+  {
+    Last(v.hosts).coordinator
+  }
+
+  predicate ValidParticipantId(c: Constants, hostid: HostId)
+  {
+    hostid < |c.hosts|-1
+  }
+
+  function ParticipantConstants(c: Constants, hostid: HostId) : ParticipantHost.Constants
+    requires Host.GroupWFConstants(c.hosts)
+    requires ValidParticipantId(c, hostid)
+  {
+    c.hosts[hostid].participant
+  }
+
+  function ParticipantVars(c: Constants, v: Variables, hostid: HostId) : ParticipantHost.Variables
+    requires Host.GroupWF(c.hosts, v.hosts)
+    requires ValidParticipantId(c, hostid)
+  {
+    v.hosts[hostid].participant
+  }
+
+  predicate AllWithDecisionAgreeWithThisOne(c: Constants, v: Variables, decision: Decision)
+    requires Host.GroupWF(c.hosts, v.hosts)
+    // I pulled this conjunction into a named predicate because Dafny warned of
+    // no trigger for the exists.
+  {
+    && (CoordinatorVars(c, v).decision.Some? ==> CoordinatorVars(c, v).decision.value == decision)
+    && (forall hostid:HostId
+      | ValidParticipantId(c, hostid) && ParticipantVars(c, v, hostid).decision.Some?
+      :: ParticipantVars(c, v, hostid).decision.value == decision)
+  }
+
+  // AC-1: All processes that reach a decision reach the same one.
+  predicate SafetyAC1(c: Constants, v: Variables)
+    requires Host.GroupWF(c.hosts, v.hosts)
+  {
+    // All hosts that reach a decision reach the same one
+    || AllWithDecisionAgreeWithThisOne(c, v, Commit)
+    || AllWithDecisionAgreeWithThisOne(c, v, Abort)
+  }
+
+  // AC2 is sort of a history predicate; we're going to ignore it.
+
+  // AC-3: The Commit decision can only be reached if all processes prefer Yes.
+  predicate SafetyAC3(c: Constants, v: Variables)
+    requires Host.GroupWF(c.hosts, v.hosts)
+  {
+    && (exists hostid:HostId
+      :: ValidParticipantId(c, hostid) && ParticipantConstants(c, hostid).preference.No?)
+      ==> AllWithDecisionAgreeWithThisOne(c, v, Abort)
+  }
+
+  // AC-4: If all processes prefer Yes, then the decision must be Commit.
+  predicate SafetyAC4(c: Constants, v: Variables)
+    requires Host.GroupWF(c.hosts, v.hosts)
+  {
+    && (forall hostid:HostId
+        | ValidParticipantId(c, hostid) :: ParticipantConstants(c, hostid).preference.Yes?)
+      ==> AllWithDecisionAgreeWithThisOne(c, v, Commit)
+  }
+
+  // AC5 is a liveness proprety, we're definitely going to ignore it.
+
+  //#instructor Player 1
+  predicate Safety(c: Constants, v: Variables)
+    requires Host.GroupWF(c.hosts, v.hosts)
+  {
+    && SafetyAC1(c, v)
+    && SafetyAC3(c, v)
+    && SafetyAC4(c, v)
+  }
+}
